

# A Pair of Diophantine Equations Involving Fibonacci Numbers

X. Chen<sup>1</sup> F. K. Kesumajana<sup>2</sup> D. Kim<sup>3</sup> L. Li<sup>4</sup> J. Yang<sup>5</sup>  
Mentors: H. V. Chu<sup>6</sup>, S. J. Miller<sup>7</sup>, C. Yao<sup>8</sup>

<sup>1</sup>mathchen314@gmail.com <sup>2</sup>nafis.khowarizmi@gmail.com

<sup>3</sup>dtkim25@berkeley.edu <sup>4</sup>zqj6pe@virginia.edu

<sup>5</sup>junchiyang1@gmail.com

<sup>6</sup>hungchu1@tamu.edu <sup>7</sup>sjm1@williams.edu <sup>8</sup>chris.yao@berkeley.edu

January 8, 2025 - Joint Mathematics Meetings

# A Pair of Equations

For relatively prime  $a, b \in \mathbb{N}$ , consider

$$ax + by = \frac{(a-1)(b-1)}{2}$$

$$ax + by + 1 = \frac{(a-1)(b-1)}{2}$$

# A Pair of Equations

For relatively prime  $a, b \in \mathbb{N}$ , consider

$$ax + by = \frac{(a-1)(b-1)}{2}$$

$$ax + by + 1 = \frac{(a-1)(b-1)}{2}$$

Theorem (Beiter (1964), extended by Chu (2020))

Exactly one of the equations has a **nonnegative integral** solution  $(x, y)$ . The solution is unique.

# A Pair of Equations

$$ax + by = \frac{(a-1)(b-1)}{2} \quad (1)$$

$$ax + by + 1 = \frac{(a-1)(b-1)}{2} \quad (2)$$

# A Pair of Equations

$$ax + by = \frac{(a-1)(b-1)}{2} \quad (1)$$

$$ax + by + 1 = \frac{(a-1)(b-1)}{2} \quad (2)$$

Define  $\Gamma : \{(a, b) \in \mathbb{N}^2 : \gcd(a, b) = 1\} \rightarrow \{1, 2\}$ :

$$\Gamma(a, b) = \begin{cases} 1, & \text{if (1) has a solution;} \\ 2, & \text{if (2) has a solution.} \end{cases}$$

# Fibonacci Numbers

$$F_1 = 1, F_2 = 1, F_3 = 2, F_4 = 3, F_5 = 5, F_6 = 8, \dots$$

# Fibonacci Numbers

$$F_1 = 1, F_2 = 1, F_3 = 2, F_4 = 3, F_5 = 5, F_6 = 8, \dots$$

$$\gcd(F_n, F_{n+1}) = 1$$

# Fibonacci Numbers

$$F_1 = 1, F_2 = 1, F_3 = 2, F_4 = 3, F_5 = 5, F_6 = 8, \dots$$

$$\gcd(F_n, F_{n+1}) = 1$$

$$a \boxed{x} + b \boxed{y} = \frac{(a-1)(b-1)}{2} \quad (1)$$

$$a \boxed{x} + b \boxed{y} + 1 = \frac{(a-1)(b-1)}{2} \quad (2)$$



# Fibonacci Numbers

$$F_1 = 1, F_2 = 1, F_3 = 2, F_4 = 3, F_5 = 5, F_6 = 8, \dots$$

$$\gcd(F_n, F_{n+1}) = 1$$

$$F_n \boxed{x} + F_{n+1} \boxed{y} = \frac{(F_n - 1)(F_{n+1} - 1)}{2} \quad (1)$$

$$F_n \boxed{x} + F_{n+1} \boxed{y} + 1 = \frac{(F_n - 1)(F_{n+1} - 1)}{2} \quad (2)$$

# Fibonacci Numbers

$$F_1 = 1, F_2 = 1, F_3 = 2, F_4 = 3, F_5 = 5, F_6 = 8, \dots$$

$$\gcd(F_n, F_{n+1}) = 1$$

$$F_n \boxed{x} + F_{n+1} \boxed{y} = \frac{(F_n - 1)(F_{n+1} - 1)}{2} \quad (1)$$

$$F_n \boxed{x} + F_{n+1} \boxed{y} + 1 = \frac{(F_n - 1)(F_{n+1} - 1)}{2} \quad (2)$$

$$\Gamma(F_n, F_{n+1}) = ?$$

# Previous work

**Chu 2020:**

$n$	3	4	5	6	7	8
$\Gamma(F_n, F_{n+1})$	2	2	2	1	1	1

# Previous work

**Chu 2020:**

$n$	3	4	5	6	7	8
$\Gamma(F_n, F_{n+1})$	2	2	2	1	1	1

$$F_{6k} \cdot \frac{F_{6k-1} - 1}{2} + F_{6k+1} \cdot \frac{F_{6k-1} - 1}{2} = \frac{(F_{6k} - 1)(F_{6k+1} - 1)}{2}$$

$$1 + F_{6k+3} \cdot \frac{F_{6k+2} - 1}{2} + F_{6k+4} \cdot \frac{F_{6k+2} - 1}{2} = \frac{(F_{6k+3} - 1)(F_{6k+4} - 1)}{2}$$

# Previous work

**Chu 2020:**

$n$	3	4	5	6	7	8
$\Gamma(F_n, F_{n+1})$	2	2	2	1	1	1

$$F_{6k} \cdot \frac{F_{6k-1} - 1}{2} + F_{6k+1} \cdot \frac{F_{6k-1} - 1}{2} = \frac{(F_{6k} - 1)(F_{6k+1} - 1)}{2}$$

$$1 + F_{6k+3} \cdot \frac{F_{6k+2} - 1}{2} + F_{6k+4} \cdot \frac{F_{6k+2} - 1}{2} = \frac{(F_{6k+3} - 1)(F_{6k+4} - 1)}{2}$$

**R. K. Davala 2023:** Identities for other famous sequences

# Previous work

**Chu 2020:**

$n$	3	4	5	6	7	8
$\Gamma(F_n, F_{n+1})$	2	2	2	1	1	1

$$F_{6k} \cdot \frac{F_{6k-1} - 1}{2} + F_{6k+1} \cdot \frac{F_{6k-1} - 1}{2} = \frac{(F_{6k} - 1)(F_{6k+1} - 1)}{2}$$

$$1 + F_{6k+3} \cdot \frac{F_{6k+2} - 1}{2} + F_{6k+4} \cdot \frac{F_{6k+2} - 1}{2} = \frac{(F_{6k+3} - 1)(F_{6k+4} - 1)}{2}$$

**R. K. Davala 2023:** Identities for other famous sequences

**Polymath Jr. 2023:** Characterize  $(a, b)$  for  $\Gamma(a, b) = 1$  or 2

# Our goals

Chu 2020:

$$F_{6k} \cdot \boxed{\frac{F_{6k-1} - 1}{2}} + F_{6k+1} \cdot \boxed{\frac{F_{6k-1} - 1}{2}} = \frac{(F_{6k} - 1)(F_{6k+1} - 1)}{2}$$

$$1 + F_{6k+3} \cdot \boxed{\frac{F_{6k+2} - 1}{2}} + F_{6k+4} \cdot \boxed{\frac{F_{6k+2} - 1}{2}} = \frac{(F_{6k+3} - 1)(F_{6k+4} - 1)}{2}$$

# Our goals

Chu 2020:

$$F_{6k} \cdot \boxed{\frac{F_{6k-1} - 1}{2}} + F_{6k+1} \cdot \boxed{\frac{F_{6k-1} - 1}{2}} = \frac{(F_{6k} - 1)(F_{6k+1} - 1)}{2}$$

$$1 + F_{6k+3} \cdot \boxed{\frac{F_{6k+2} - 1}{2}} + F_{6k+4} \cdot \boxed{\frac{F_{6k+2} - 1}{2}} = \frac{(F_{6k+3} - 1)(F_{6k+4} - 1)}{2}$$

$$\Gamma(F_n^2, F_{n+1}^2) = ?$$



# Our goals

Chu 2020:

$$F_{6k} \cdot \boxed{\frac{F_{6k-1} - 1}{2}} + F_{6k+1} \cdot \boxed{\frac{F_{6k-1} - 1}{2}} = \frac{(F_{6k} - 1)(F_{6k+1} - 1)}{2}$$

$$1 + F_{6k+3} \cdot \boxed{\frac{F_{6k+2} - 1}{2}} + F_{6k+4} \cdot \boxed{\frac{F_{6k+2} - 1}{2}} = \frac{(F_{6k+3} - 1)(F_{6k+4} - 1)}{2}$$

$$\Gamma(F_n^2, F_{n+1}^2) = ?$$

Are there similar identities for Fibonacci squared?

# Fibonacci Squared - The Data

$$ax + by = \frac{(a-1)(b-1)}{2} \quad (1)$$

$$ax + by + 1 = \frac{(a-1)(b-1)}{2} \quad (2)$$

$n$	$F_n^2$	$F_{n+1}^2$	$x$	$y$	$\Gamma(F_n^2, F_{n+1}^2)$
2	1	4	0	0	(1)
3	4	9	3	0	(1)
4	9	25	5	2	(2)
5	25	64	20	4	(1)
6	64	169	51	12	(1)
7	169	441	83	52	(2)

Table: Fibonacci squared

# Fibonacci Squared - The Data

$n$	$F_n^2$	$F_{n+1}^2$	$x$	$y$	$\Gamma(F_n^2, F_{n+1}^2)$	$F_n^2 - x - y$
2	1	4	0	0	(1)	<b>1</b>
3	4	9	3	0	(1)	<b>1</b>
4	9	25	5	2	(2)	2
5	25	64	20	4	(1)	<b>1</b>
6	64	169	51	12	(1)	<b>1</b>
7	169	441	83	52	(2)	34
8	441	1156	356	84	(1)	<b>1</b>
9	1156	3025	935	220	(1)	<b>1</b>
10	3025	7921	1513	934	(2)	578
$\vdots$	$\vdots$	$\vdots$	$\vdots$	$\vdots$	$\vdots$	$\vdots$
13	54289	142129	27143	16776	(2)	10370

Table: Fibonacci Squared Pattern

# Fibonacci Squared - The Data

$n$	$F_n^2$	$F_{n+1}^2$	$x$	$y$	$\Gamma(F_n^2, F_{n+1}^2)$	$F_n^2 - x - y$
2	1	4	0	0	(1)	1
3	4	9	3	0	(1)	1
4	<b>9</b>	25	<b>5</b>	2	(2)	2
5	25	64	20	4	(1)	1
6	64	169	51	12	(1)	1
7	<b>169</b>	441	<b>83</b>	52	(2)	34
8	441	1156	356	84	(1)	1
9	1156	3025	935	220	(1)	1
10	<b>3025</b>	7921	<b>1513</b>	934	(2)	578
$\vdots$	$\vdots$	$\vdots$	$\vdots$	$\vdots$	$\vdots$	$\vdots$
13	<b>54289</b>	142129	<b>27143</b>	16776	(2)	10370

Table: Fibonacci Squared Pattern

# Identities for Fibonacci Squared

## Theorem

For  $n \geq 7$  with  $n \equiv 1 \pmod{6}$ , the following holds

$$F_n^2 \cdot \frac{F_n^2 - 3}{2} + F_{n+1}^2 \cdot \frac{F_n^2 - F_{n-1}^2 - 1}{2} + 1 = \frac{(F_n^2 - 1)(F_{n+1}^2 - 1)}{2}.$$

# Identities for Fibonacci Squared

## Theorem

For  $n \geq 7$  with  $n \equiv 1 \pmod{6}$ , the following holds

$$F_n^2 \cdot \left\lfloor \frac{F_n^2 - 3}{2} \right\rfloor + F_{n+1}^2 \cdot \left\lfloor \frac{F_n^2 - F_{n-1}^2 - 1}{2} \right\rfloor + 1 = \frac{(F_n^2 - 1)(F_{n+1}^2 - 1)}{2}.$$

## Theorem

For  $n \geq 1$  with  $n \equiv 4 \pmod{6}$ , the following holds

$$F_n^2 \cdot \left\lfloor \frac{F_n^2 + 1}{2} \right\rfloor + F_{n+1}^2 \cdot \left\lfloor \frac{F_n^2 - F_{n-1}^2 - 1}{2} \right\rfloor + 1 = \frac{(F_n^2 - 1)(F_{n+1}^2 - 1)}{2}.$$

# Identities for Fibonacci Squared

## Theorem

For  $n \geq 1$  with  $n \equiv 0, 2, 3, 5 \pmod{6}$ , the following holds

$$F_n^2 \cdot \left( F_n^2 - \frac{F_{n-1}^2 + 1}{2} \right) + F_{n+1}^2 \cdot \frac{F_{n-1}^2 - 1}{2} = \frac{(F_n^2 - 1)(F_{n+1}^2 - 1)}{2}.$$

# Proof

## Theorem

For  $n \geq 1$  with  $n \equiv 0, 2, 3, 5 \pmod{6}$ , the following identity holds

$$F_n^2 \cdot \left( F_n^2 - \frac{F_{n-1}^2 + 1}{2} \right) + F_{n+1}^2 \cdot \frac{F_{n-1}^2 - 1}{2} = \frac{(F_n^2 - 1)(F_{n+1}^2 - 1)}{2}$$



# Proof

## Theorem

For  $n \geq 1$  with  $n \equiv 0, 2, 3, 5 \pmod{6}$ , the following identity holds

$$F_n^2 \cdot \left( F_n^2 - \frac{F_{n-1}^2 + 1}{2} \right) + F_{n+1}^2 \cdot \frac{F_{n-1}^2 - 1}{2} = \frac{(F_n^2 - 1)(F_{n+1}^2 - 1)}{2}$$

## Proof:

$$F_n = F_{n+1} - F_{n-1}$$

# Proof

## Theorem

For  $n \geq 1$  with  $n \equiv 0, 2, 3, 5 \pmod{6}$ , the following identity holds

$$F_n^2 \cdot \left( F_n^2 - \frac{F_{n-1}^2 + 1}{2} \right) + F_{n+1}^2 \cdot \frac{F_{n-1}^2 - 1}{2} = \frac{(F_n^2 - 1)(F_{n+1}^2 - 1)}{2}$$

## Proof:

$$F_n = F_{n+1} - F_{n-1} \implies F_n^2 - F_{n-1}^2 - F_{n+1}^2 = -2F_{n-1}F_{n+1}$$

# Proof

## Theorem

For  $n \geq 1$  with  $n \equiv 0, 2, 3, 5 \pmod{6}$ , the following identity holds

$$F_n^2 \cdot \left( F_n^2 - \frac{F_{n-1}^2 + 1}{2} \right) + F_{n+1}^2 \cdot \frac{F_{n-1}^2 - 1}{2} = \frac{(F_n^2 - 1)(F_{n+1}^2 - 1)}{2}$$

## Proof:

$$F_n = F_{n+1} - F_{n-1} \implies F_n^2 - F_{n-1}^2 - F_{n+1}^2 = -2F_{n-1}F_{n+1}$$

$$(F_{n-1}F_{n+1} - F_n^2)^2 = ((-1)^n)^2 \quad (\text{Cassini's Identity})$$

# Proof

## Theorem

For  $n \geq 1$  with  $n \equiv 0, 2, 3, 5 \pmod{6}$ , the following identity holds

$$F_n^2 \cdot \left( F_n^2 - \frac{F_{n-1}^2 + 1}{2} \right) + F_{n+1}^2 \cdot \frac{F_{n-1}^2 - 1}{2} = \frac{(F_n^2 - 1)(F_{n+1}^2 - 1)}{2}$$

## Proof:

$$F_n = F_{n+1} - F_{n-1} \implies F_n^2 - F_{n-1}^2 - F_{n+1}^2 = -2F_{n-1}F_{n+1}$$

$$(F_{n-1}F_{n+1} - F_n^2)^2 = ((-1)^n)^2 \quad (\text{Cassini's Identity})$$

$$\implies F_n^4 - 2F_n^2F_{n-1}F_{n+1} + F_{n-1}^2F_{n+1}^2 = 1$$

# Proof

$$F_n^2 - F_{n-1}^2 - F_{n+1}^2 = -2F_{n-1}F_{n+1}$$

$$F_n^4 - 2F_n^2F_{n-1}F_{n+1} + F_{n-1}^2F_{n+1}^2 = 1$$

$$\implies 2F_n^4 - F_n^2F_{n-1}^2 - F_n^2F_{n+1}^2 + F_{n-1}^2F_{n+1}^2 = 1$$

# Proof

$$F_n^2 - F_{n-1}^2 - F_{n+1}^2 = -2F_{n-1}F_{n+1}$$

$$F_n^4 - 2F_n^2F_{n-1}F_{n+1} + F_{n-1}^2F_{n+1}^2 = 1$$

$$\implies 2F_n^4 - F_n^2F_{n-1}^2 - F_n^2F_{n+1}^2 + F_{n-1}^2F_{n+1}^2 = 1$$

$$(2F_n^2 - F_{n-1}^2 - 1) \cdot F_n^2 + (F_{n-1}^2 - 1) \cdot F_{n+1}^2 = (F_n^2 - 1)(F_{n+1}^2 - 1)$$

# Proof

$$F_n^2 - F_{n-1}^2 - F_{n+1}^2 = -2F_{n-1}F_{n+1}$$

$$F_n^4 - 2F_n^2F_{n-1}F_{n+1} + F_{n-1}^2F_{n+1}^2 = 1$$

$$\implies 2F_n^4 - F_n^2F_{n-1}^2 - F_n^2F_{n+1}^2 + F_{n-1}^2F_{n+1}^2 = 1$$

$$(2F_n^2 - F_{n-1}^2 - 1) \cdot F_n^2 + (F_{n-1}^2 - 1) \cdot F_{n+1}^2 = (F_n^2 - 1)(F_{n+1}^2 - 1)$$

$$\left(F_n^2 - \frac{F_{n-1}^2 + 1}{2}\right) \cdot F_n^2 + \left(\frac{F_{n-1}^2 - 1}{2}\right) \cdot F_{n+1}^2 = \frac{(F_n^2 - 1)(F_{n+1}^2 - 1)}{2}$$

# Fibonacci Cubed - The Data

What about Fibonacci cubed?



# Fibonacci Cubed - The Data

What about Fibonacci cubed?

$n$	$F_n^3$	$F_{n+1}^3$	$x_n$	$y_n$	$\Gamma(F_n^3, F_{n+1}^3)$
2	1	8	0	0	(1)
3	8	27	8	1	(1)
4	27	125	18	9	(2)
5	125	512	106	36	(1)
6	512	2197	405	161	(2)
7	2197	9261	1791	673	(1)

Table: Fibonacci cubed

# Fibonacci Cubed - The Data

What about Fibonacci cubed?

$n$	$F_n^3$	$F_{n+1}^3$	$x_n$	$y_n$	$\Gamma(F_n^3, F_{n+1}^3)$
2	1	8	0	0	(1)
3	8	27	8	1	(1)
4	27	125	18	9	(2)
5	125	512	106	36	(1)
6	512	2197	405	161	(2)
7	2197	9261	1791	673	(1)

Table: Fibonacci cubed

$$x_4 = 3^3 - x_3 - 1; \quad y_4 = y_3 + 2^3$$

$$x_5 = 5^3 - x_4 - 1; \quad y_5 = y_4 + 3^3$$

$$x_6 = 8^3 - x_5 - 1; \quad y_6 = y_5 + 5^3$$

# Fibonacci Cubed - The Data

$$\begin{cases} x_n &= F_n^3 - x_{n-1} - 1 \\ y_n &= y_{n-1} + F_{n-1}^3. \end{cases}$$

# Fibonacci Cubed - The Data

$$\begin{cases} x_n &= F_n^3 - x_{n-1} - 1 \\ y_n &= y_{n-1} + F_{n-1}^3. \end{cases}$$

## Theorem

Let  $n \in \mathbb{N}$  with  $n \geq 2$ . The following hold

$$\begin{aligned} \left[ \sum_{k=1}^{2n-1} (-1)^{k-1} F_k^3 \right] F_{2n-1}^3 + \left( \sum_{k=2}^{2n-2} F_k^3 \right) F_{2n}^3 &= \frac{(F_{2n-1}^3 - 1)(F_{2n}^3 - 1)}{2}, \\ 1 + \left[ \sum_{k=1}^{2n} (-1)^k F_k^3 - 1 \right] F_{2n}^3 + \left( \sum_{k=2}^{2n-1} F_k^3 \right) F_{2n+1}^3 &= \frac{(F_{2n}^3 - 1)(F_{2n+1}^3 - 1)}{2}. \end{aligned}$$

# Proof Sketch

Frontczak's formulas (2018) to replace sums of Fibonacci cubes:

$$\begin{aligned}
 & \left( \frac{F_{6n}}{4} - \frac{F_{6n-3}}{4} - F_{2n}^3 + F_{2n-1}^3 - \frac{1}{2} \right) F_{2n-1}^3 \\
 & + \left( \frac{F_{6n-3}}{4} + \frac{F_{6n-6}}{4} - F_{2n-1}^3 - F_{2n-2}^3 - \frac{1}{2} \right) F_{2n}^3 \\
 & = \frac{(F_{2n-1}^3 - 1)(F_{2n}^3 - 1)}{2}
 \end{aligned}$$

## Proof Sketch

Frontczak's formulas (2018) to replace sums of Fibonacci cubes:

$$\begin{aligned} & \left( \frac{F_{6n}}{4} - \frac{F_{6n-3}}{4} - F_{2n}^3 + F_{2n-1}^3 - \frac{1}{2} \right) F_{2n-1}^3 \\ & + \left( \frac{F_{6n-3}}{4} + \frac{F_{6n-6}}{4} - F_{2n-1}^3 - F_{2n-2}^3 - \frac{1}{2} \right) F_{2n}^3 \\ & = \frac{(F_{2n-1}^3 - 1)(F_{2n}^3 - 1)}{2} \end{aligned}$$

Equivalently, we need to prove

$$\begin{aligned} (F_{6n} - F_{6n-3})F_{2n-1}^3 + 4F_{2n-1}^6 + (F_{6n-3} + F_{6n-6})F_{2n}^3 \\ - 4F_{2n-2}^3 - 10F_{2n-1}^3F_{2n}^3 = 2 \end{aligned}$$

# Proof Sketch

$$F_{3n} = 5F_n^3 + 3(-1)^n F_n$$

# Proof Sketch

$$F_{3n} = 5F_n^3 + 3(-1)^n F_n$$

$$\implies (F_{6n} - F_{6n-3}) F_{2n-1}^3 = (5F_{2n}^3 + 3F_{2n} - 5F_{2n-1}^3 + 3F_{2n-1}) F_{2n-1}^3$$



# Proof Sketch

$$F_{3n} = 5F_n^3 + 3(-1)^n F_n$$

$$\implies (F_{6n} - F_{6n-3}) F_{2n-1}^3 = (5F_{2n}^3 + 3F_{2n} - 5F_{2n-1}^3 + 3F_{2n-1}) F_{2n-1}^3$$

$$F_{2n-2} F_{2n} = (-1)^{2n-1} + F_{2n-1}^2 = -1 + F_{2n-1}^2 \quad (\text{Cassini's Identity})$$

# Proof Sketch

$$F_{3n} = 5F_n^3 + 3(-1)^n F_n$$

$$\implies (F_{6n} - F_{6n-3}) F_{2n-1}^3 = (5F_{2n}^3 + 3F_{2n} - 5F_{2n-1}^3 + 3F_{2n-1}) F_{2n-1}^3$$

$$F_{2n-2} F_{2n} = (-1)^{2n-1} + F_{2n-1}^2 = -1 + F_{2n-1}^2 \quad (\text{Cassini's Identity})$$

$$\implies (F_{6n} - F_{6n-3}) F_{2n-1}^3 + 4F_{2n-1}^6 + (F_{6n-3} + F_{6n-6}) F_{2n}^3 - 4F_{2n-2}^3 - 10F_{2n-1}^3 F_{2n}^3 = 2$$

# Another Pair of Diophantine Equations

## Theorem

Given  $a, b \in \mathbb{N}$  with  $(a, b) = 1$ , consider the two following equations.

$$x^a + y^b = \frac{(a-1)(b-1)}{2},$$
$$1 + x^a + y^b = \frac{(a-1)(b-1)}{2}.$$

Exactly one of the equations above has a **nonnegative integral** solution  $(x, y)$ , and the solution is unique.

## Another Pair of Diophantine Equations

$(a, b) = (7, 8)$  gives  $(x, y) = (3, 0)$ :

$$3 \cdot 7 + 0 \cdot 8 = \frac{(7-1)(8-1)}{2}.$$

# Another Pair of Diophantine Equations

$(a, b) = (7, 8)$  gives  $(x, y) = (3, 0)$ :

$$3 \cdot 7 + 0 \cdot 8 = \frac{(7-1)(8-1)}{2}.$$

Can we find a pair of equations that give only **positive** solutions?

# Another Pair of Diophantine Equations

## Theorem

Given  $a, b \in \mathbb{N}$  with  $(a, b) = 1$ , consider the two following equations

$$x\textcolor{red}{a} + y\textcolor{blue}{b} = \frac{(\textcolor{red}{a}-1)(\textcolor{blue}{b}-1)}{2} + (\textcolor{red}{a} + \textcolor{blue}{b}),$$
$$1 + x\textcolor{red}{a} + y\textcolor{blue}{b} = \frac{(\textcolor{red}{a}-1)(\textcolor{blue}{b}-1)}{2} + (\textcolor{red}{a} + \textcolor{blue}{b}).$$

Exactly one of the equations above has a **positive integral** solution  $(x, y)$ , and the solution is unique.

# Another Pair of Diophantine Equations

$$(a, b) = (7, 8):$$

$$\text{Old:} \quad 3 \cdot 7 + 0 \cdot 8 = \frac{(7-1)(8-1)}{2}$$

$$\text{New:} \quad 4 \cdot 7 + 1 \cdot 8 = \frac{(7-1)(8-1)}{2} + (7+8)$$

$$(3, 0) \rightarrow (3+1, 0+1)$$

# Another Pair of Diophantine Equations

## Theorem

Given  $a, b \in \mathbb{N}$  with  $(a, b) = 1$ ,  $b \geq 2$ , and  $(a + 1)b \equiv 0 \pmod{2}$ , consider the two following equations

$$xa + yb = \frac{(a + 1)b}{2} + 1, \quad (3)$$

$$xa + yb = \frac{(a + 1)b}{2} - 1. \quad (4)$$

Exactly one of the two equations has a **positive integral** solution  $(x, y)$ , and the solution is unique.



# Another Pair of Diophantine Equations

## Theorem

Given  $a, b \in \mathbb{N}$  with  $(a, b) = 1$ ,  $b \geq 2$ , and  $(a + 1)b \equiv 0 \pmod{2}$ , consider the two following equations

$$x^a + y^b = \frac{(a+1)b}{2} + 1, \quad (3)$$

$$x^a + y^b = \frac{(a+1)b}{2} - 1. \quad (4)$$

Exactly one of the two equations has a **positive integral** solution  $(x, y)$ , and the solution is unique.

Define  $\Gamma' : \{(a, b) : (a, b) = 1, b \geq 2, 2 \text{ divides } (a + 1)b\} \rightarrow \{1, 2\}$ :

$$\Gamma'(a, b) = \begin{cases} 1, & \text{if (3) has a solution;} \\ 2, & \text{if (4) has a solution.} \end{cases}$$

# Another Pair of Diophantine Equations

Asymmetric: possible that  $\Gamma'(a, b) \neq \Gamma'(b, a)$ .

$(a, b) = (3, 5)$  and  $(a, b) = (5, 3)$

$$2 \cdot 3 + 1 \cdot 5 = \frac{(3+1)5}{2} + 1$$

$$1 \cdot 5 + 1 \cdot 3 = \frac{(5+1)3}{2} - 1$$

# What's next

Examine higher powers of Fibonacci numbers

# What's next

Examine higher powers of Fibonacci numbers

Explore  $\Gamma(F_n^i, F_{n+1}^j)$  for  $i \neq j$

# What's next

Examine higher powers of Fibonacci numbers

Explore  $\Gamma(F_n^i, F_{n+1}^j)$  for  $i \neq j$

Characterize when  $\Gamma'(a, b) \neq \Gamma'(b, a)$